Coq: QoL changes in InductiveDefinitions

theories/InductiveDefinitions.v
@@ -1,7 +1,7 @@
 Require Import Base Syntax Semantics.
 
 Section inductive_definition_set.
-  Context {Σ : signature}.
+  Context (Σ : signature).
   
   Record production :=
     mkProd {
@@ -10,28 +10,33 @@ Section inductive_definition_set.
         indcons : IndPredS Σ;
         indargs : vec (term Σ) (indpred_ar indcons);
       }.
-
+  
   Definition IndDefSet := production -> Prop.
 End inductive_definition_set.
 
+Arguments mkProd {Σ}.
+Arguments preds {Σ}.
+Arguments indpreds {Σ}.
+Arguments indcons {Σ}.
+Arguments indargs {Σ}.
+
 Section definition_set_operator.
   Context {Σ : signature}.
-  Context {M : structure Σ}.
-  Context {Φ : @IndDefSet Σ}.
-  Let D := domain M.             
-  (*
-    D^k ≡ vec D k
-    Pow(D^k) ≡ vec D k -> Prop
-    Pow(D^1) × ... × Pow(D^k) ≡ ∀ P, vec D (indpred_ar P) -> Prop
-   *)
+  Context (Φ : IndDefSet Σ).
+  Context (M : structure Σ).
 
-  (* Definition Φ_P (* Φ_i *) (P : IndPredS Σ): production -> Prop := *)
-  (*   fun pr => Φ pr /\ indcons pr = P. *)
+  (* interpretation of inductive predicates *)
+  Definition InterpInd := forall P : IndPredS Σ, vec M (indpred_ar P) -> Prop.
+
+  Definition subset (U V : InterpInd) := forall P v, U P v -> V P v.
+  Notation "U ⊑ V" := (subset U V) (at level 11).
   
-  Definition φ_pr (* φ_{i, r} *)
-    (pr : production)
-    (args : forall P : IndPredS Σ, vec D (indpred_ar P) -> Prop)
-    (ds : vec D (indpred_ar (indcons pr)))
+  Definition monotone (F : InterpInd -> InterpInd) := forall U V : InterpInd, U ⊑ V -> F U ⊑ F V.
+  
+  Definition φ_pr
+    (pr : production Σ)
+    (args : InterpInd)
+    (ds : vec M (indpred_ar (indcons pr)))
     : Prop :=
         exists (ρ : env M),
         (forall Q us, List.In (Q; us) (preds pr) ->
@@ -40,24 +45,21 @@ Section definition_set_operator.
                     args P (V.map (eval ρ) ts)) /\
           ds = V.map (eval ρ) (indargs pr).
 
-  Definition φ_P (* φ_i *)
+  Definition φ_P
     (P : IndPredS Σ)
-    (args : forall P : IndPredS Σ, vec D (indpred_ar P) -> Prop)
-    : vec D (indpred_ar P) -> Prop.
+    (args : InterpInd)
+    : vec M (indpred_ar P) -> Prop.
     refine (fun ds => _).
-    refine (@ex production (fun pr => _)).
+    refine (@ex (production Σ) (fun pr => _)).
     refine (@ex (P = indcons pr /\ Φ pr) (fun '(conj Heq HΦ) => _)).
     rewrite Heq in ds.
     exact (φ_pr pr args ds).
   Defined.
   
-  Definition φ_Φ (args : forall P : IndPredS Σ, vec D (indpred_ar P) -> Prop)
-    : forall P : IndPredS Σ, vec D (indpred_ar P) -> Prop :=
+  Definition φ_Φ (args : InterpInd) : InterpInd :=
     fun P => φ_P P args.
-
-  Proposition φ_Φ_monotone : forall (f g : forall P, vec D (indpred_ar P) -> Prop),
-      (forall P v, f P v -> g P v) ->
-      (forall P v, φ_Φ f P v -> φ_Φ g P v).
+  
+  Proposition φ_Φ_monotone : monotone φ_Φ.
   Proof.
     intros f g Hle P v Hφ.
     unfold φ_Φ, φ_P in *.
@@ -70,49 +72,45 @@ Section definition_set_operator.
     - intros PP ts HIn. apply Hle. apply Hindpreds; auto.
     - apply Hcons.
   Qed.
-End definition_set_operator.
 
-Section approximants.
-  Context {Σ : signature} {M : structure Σ}.
-  Context {Φ : @IndDefSet Σ}.
-
-  Fixpoint φ_Φ_n P (α : nat) (v : vec M (indpred_ar P)) : Prop :=
+  Fixpoint φ_Φ_n (α : nat) : InterpInd :=
     match α with
-    | 0 => False
-    | S α => @φ_Φ Σ M Φ (fun P => φ_Φ_n P α) P v
+    | 0 => fun _ _ => False
+    | S α => φ_Φ (φ_Φ_n α)
     end.
 
-  Corollary (* 2.2.10 *) cor : forall α P v,
-      φ_Φ_n P (S α) v <-> @φ_Φ Σ M Φ (fun P => φ_Φ_n P α) P v.
+  Lemma φ_Φ_n_succ : forall α : nat, φ_Φ_n α ⊑ φ_Φ_n (S α).
   Proof.
-    intros α P v. cbn; split; auto.
+    induction α as [| α IH].
+    - inversion 1.
+    - apply φ_Φ_monotone, IH.
   Qed.
-    
+      
+  Lemma φ_Φ_n_monotone : forall α β : nat, α <= β -> φ_Φ_n α ⊑ φ_Φ_n β.
+  Proof.
+    intros α β Hle; induction Hle as [| β _ IH].
+    - red; auto.
+    - pose proof (φ_Φ_n_succ β); red; auto.
+  Qed.
+      
   Definition approximant_of (P : IndPredS Σ)
     : nat -> vec M (indpred_ar P) -> Prop :=
-    φ_Φ_n P.
+    fun α => φ_Φ_n α P.
 
-  Lemma zeroth_approximant_empty :
-    forall P v, ~approximant_of P 0 v.
+  Proposition approximant_succ : forall α P v,
+      approximant_of P α v -> approximant_of P (S α) v.
   Proof.
-    intros P v Happrox; inversion Happrox.
-  Qed.
-
-  Proposition (* 2.2.9 *) approximant_succ : forall α P v, approximant_of P α v -> approximant_of P (S α) v.
-  Proof.
-    unfold approximant_of; induction α; intros P v H.
-    - inversion H.
-    - apply φ_Φ_monotone with (fun P => φ_Φ_n P α); auto.
+    now apply φ_Φ_n_succ.
   Qed.
   
-  Lemma approximant_monotone : forall α β, α < β -> forall P v, approximant_of P α v -> approximant_of P β v.
+  Lemma approximant_monotone : forall α β, α <= β -> forall P v,
+        approximant_of P α v -> approximant_of P β v.
   Proof.
-    unfold approximant_of. intros α β Hle P v Hφ.
-    induction Hle; now apply approximant_succ.
+    now apply φ_Φ_n_monotone.
   Qed.  
       
-  Lemma approximant_characterization : forall α P v,
-      φ_Φ_n P α v <-> exists β, β < α /\ @φ_Φ Σ M Φ (fun P => φ_Φ_n P β) P v.
+  Lemma approximation_characterization : forall α P v,
+      φ_Φ_n α P v <-> exists β, β < α /\ φ_Φ (φ_Φ_n β) P v.
   Proof.
     intros α P v; split; intros H.
     - induction α.
@@ -120,45 +118,26 @@ Section approximants.
       + exists α; split; [apply le_n | apply H].
     - destruct H as [β [Hle Hφ]]; induction Hle.
       + apply Hφ.
-      + now apply approximant_succ.
+      + now apply φ_Φ_n_succ.
   Qed.
 
-  Lemma lema_iza_cor_2_2_10 :   (* nije prava lema, napisana je kao komentar *)
-    forall α, (forall P v, φ_Φ_n P (S α) v <-> φ_Φ_n P α v) <->
-           (forall P v, @φ_Φ Σ M Φ (fun P => φ_Φ_n P α) P v -> φ_Φ_n P α v).
-  Proof.
-    intros α; split; intros H.
-    - intros P v H1. apply H. apply H1.
-    - intros P v; split.
-      + intros H1. apply H. apply H1.
-      + intros H1. cbn. now apply approximant_succ.
-  Qed.
+  Definition φ_Φ_ω : InterpInd := fun P v => exists α, φ_Φ_n α P v.
   
-  Definition φ_Φ_ω P v := exists α, φ_Φ_n P α v.
-
-  Lemma φ_Φ_ω_characterization : forall P v, φ_Φ_ω P v <-> exists α, @φ_Φ Σ M Φ (fun P => φ_Φ_n P α) P v.
+  Definition prefixed (U : InterpInd) := φ_Φ U ⊑ U.
+  Definition least (P : InterpInd -> Prop) (U : InterpInd) := P U /\ (forall V, P V -> U ⊑ V).
+  
+  Lemma φ_Φ_ω_least_prefixed : least prefixed φ_Φ_ω.
   Proof.
-    intros P v; split; intros [α Hφ].
-    - destruct α.
-      + inversion Hφ.
-      + exists α. apply Hφ.
-    - exists (S α). apply Hφ.
-  Qed.
-
-  Import ListNotations.
-
-  Section lemma_2_2_11.         (* uses proof irrelevance *)
-    Lemma ω_prefixed : forall P v, @φ_Φ Σ M Φ φ_Φ_ω P v -> φ_Φ_ω P v.
-    Proof.
-      intros P y H.
+    split.
+    - intros P v H.
       unfold φ_Φ, φ_P, φ_pr in H;
-      destruct H as (pr & [Heq Hpr] & (ρ & H1 & H2 & H3)).
-      unfold eq_rect in H3; subst P; subst y.
-      assert (Hsup : exists α, forall P ts, In (P; ts) (indpreds pr) -> φ_Φ_n P α (V.map (eval ρ) ts)).
+        destruct H as (pr & [Heq Hpr] & (ρ & H1 & H2 & H3)).
+      unfold eq_rect in H3; subst P; subst v.
+      assert (Hsup : exists α, forall P ts, In (P; ts) (indpreds pr) -> φ_Φ_n α P (V.map (eval ρ) ts)).
       {
         induction (indpreds pr).
-        - exists 0. intros. contradiction.
-        - destruct a. pose proof (H2 x t).
+        + exists 0. intros. contradiction.
+        + destruct a. pose proof (H2 x t).
           assert (In (x; t) ((x; t) :: l)) by now left.
           apply H in H0. destruct H0 as [α Hα].
           assert (IH_help : forall P ts, In (P; ts) l -> φ_Φ_ω P (V.map (eval ρ) ts)).
@@ -168,14 +147,14 @@ Section approximants.
           exists (S (max α β)).
           intros P ts Hin.
           inversion Hin.
-          + apply approximant_monotone with α.
-            * auto with arith.
-            * apply EqdepFacts.eq_sigT_fst in H0 as HHH.
-              subst x. unfold approximant_of.
-              apply inj_pair2 in H0 as HH. subst t. assumption.
-          + apply approximant_monotone with β.
-            * auto with arith.
-            * clear Hin. now apply Hβ.                                
+          * apply approximant_monotone with α.
+            -- auto with arith.
+            -- apply EqdepFacts.eq_sigT_fst in H0 as HHH.
+               subst x. unfold approximant_of.
+               apply inj_pair2 in H0 as HH. subst t. assumption.
+          * apply approximant_monotone with β.
+            -- auto with arith.
+            -- clear Hin. now apply Hβ.                                
       }
       destruct Hsup as [κ Hsup].
       exists (S κ).
@@ -183,41 +162,20 @@ Section approximants.
       unfold φ_P.
       exists pr, (conj eq_refl Hpr).
       unfold φ_pr. exists ρ; split; auto.
-    Qed.
-
-    Lemma ω_least : forall args, (forall P v, @φ_Φ Σ M Φ args P v -> args P v) ->
-                            forall P v, φ_Φ_ω P v -> args P v.
-    Proof.
-      intros args (* prefixed point *) Hprefixed P v Hω.
+    - intros args Hprefixed P v Hω.
       destruct Hω as [α Hφ].
-      enough (H : forall m, @φ_Φ Σ M Φ (fun P => φ_Φ_n P m) P v ->
-                       @φ_Φ Σ M Φ args P v).
-      - apply Hprefixed. apply H with α.
-        apply approximant_succ. apply Hφ.
-      - intros m. apply φ_Φ_monotone. induction m; intros Q u HQ.
-        + inversion HQ.
-        + apply Hprefixed. eapply φ_Φ_monotone.
-          2:{ apply HQ. }
-          intros. cbn in *. fold φ_Φ_n in H. apply IHm. apply H.
-    Qed.    
-  End lemma_2_2_11.
-End approximants.
+      enough (H: forall β, φ_Φ (φ_Φ_n β) P v -> φ_Φ args P v).
+      + now apply Hprefixed, (H α), φ_Φ_n_succ.
+      + intros β; apply φ_Φ_monotone. induction β as [| β IH].
+        * inversion 1.
+        * cbn; unfold prefixed in Hprefixed.
+          apply φ_Φ_monotone in IH. red; auto.
+  Qed.
+End definition_set_operator.
 
-Definition standard_model
-  (Σ : signature) (Φ: @IndDefSet Σ) (M : structure Σ) : Prop :=
-  forall (P : IndPredS Σ) ts, interpIP P ts <-> @φ_Φ_ω Σ M Φ P ts.
-
-Lemma standard_model_inductive_implication :
-  forall Σ (Φ : @IndDefSet Σ) (M : structure Σ) (ρ : env M) (pr : @production Σ),
-    Φ pr ->
-    standard_model Σ Φ M ->
-    (forall Q us, In (Q; us) (preds pr) -> interpP Q (V.map (eval ρ) us)) ->
-    (forall P ts, In (P; ts) (indpreds pr) -> interpIP P (V.map (eval ρ) ts)) ->
-    ρ ⊨ (FIndPred (indcons pr) (indargs pr)).
-Proof.
-  intros; cbn in *.
-  apply H0. apply ω_prefixed.
-  unfold φ_Φ, φ_P; exists pr, (conj eq_refl H); cbn.
-  unfold φ_pr; exists ρ; repeat split; auto.
-  intros. apply H0. auto.
-Qed.
+Section standard_model.
+  Context {Σ : signature}.
+  
+  Definition standard_model (Φ: IndDefSet Σ) (M : structure Σ) : Prop :=
+    forall (P : IndPredS Σ) ts, interpIP P ts <-> φ_Φ_ω Φ M P ts.
+End standard_model.
